num/W/W2/W2_add_c_spec.v
@@ -1,0 +1,35 @@
+Require Import ZArith.
+Open Local Scope Z_scope.
+Require Import W2_basic.
+Open Local Scope w2_scope.
+Require Import W2_add.
+
+
+Lemma w2_add_c_spec : forall x y, [+|w2_add_c x y|] = [|x|] + [|y|].
+Proof
+fun x y =>
+ match x as x return [+|w2_add_c x y|] = [|x|] + [|y|] with
+ | OO => refl_equal [|y|]
+ | OI => 
+    match y as y return [+|w2_add_c OI y|] = [|OI|] + [|y|] with
+    | OO => refl_equal (1)
+    | OI => refl_equal (2)
+    | IO => refl_equal (3)
+    | II => refl_equal (4)
+    end
+ | IO => 
+    match y as y return [+|w2_add_c IO y|] = [|IO|] + [|y|] with
+    | OO => refl_equal (2)
+    | OI => refl_equal (3)
+    | IO => refl_equal (4)
+    | II => refl_equal (5)
+    end
+ | II => 
+    match y as y return [+|w2_add_c II y|] = [|II|] + [|y|] with
+    | OO => refl_equal (3)
+    | OI => refl_equal (4)
+    | IO => refl_equal (5)
+    | II => refl_equal (6)
+    end
+ end.
+
