num/W/W2/W2_div.v
@@ -1,0 +1,51 @@
+Require Import ZArith.
+Open Local Scope Z_scope.
+Require Import W2_basic.
+Open Local Scope w2_scope.
+
+
+Require Import W2_compare.
+Require Import W2_add.
+Require Import W2_sub.
+
+(* ** Division ** *)
+
+Definition w2_div_wB x y :=
+ match y with
+ | OO => (C0 OO, OO)
+ | OI => (C0 OO, OO)
+ | IO =>
+    match x with
+    | OO => (C0 OO, OO)
+    | OI => (C0 IO, OO)
+    | IO => (C1 OO, OO)
+    | II => (C1 IO, OO)
+   end
+ | II =>
+    match x with
+    | OO => (C0 OO, OO)
+    | OI => (C0 OI, OI)
+    | IO => (C0 IO, IO)
+    | II => (C1 OO, OO)
+   end
+ end.
+
+Definition w2_div21 a1 a2 b :=
+ let (q,s) := w2_div_wB a1 b in
+ match w2_add_c s a2 with
+ | C0 r =>
+   match w2_compare r b with
+   | Eq => (w2_carry_succ_c q, OO)
+   | Lt => (q, r)
+   | Gt => (w2_carry_succ_c q, w2_sub r b)
+   end
+ | C1 r =>
+   let q := w2_carry_succ_c q in
+   let r' := w2_sub r b in
+   match w2_compare r' b with
+   | Eq => (w2_carry_succ_c q, OO)
+   | Lt => (q, r')
+   | Gt => (w2_carry_succ_c q, w2_sub r' b)
+   end
+ end.
+
