num/W/W2/W2_mul_spec.v
@@ -1,0 +1,31 @@
+Require Import ZArith.
+Open Local Scope Z_scope.
+Require Import W2_basic.
+Require Import W2_basic_spec.
+Open Local Scope w2_scope.
+Require Import W2_mul.
+
+
+Require Import ZDivModAux.
+Require Import W2_mul_c_spec.
+Open Local Scope Z_scope.
+
+
+Lemma w2_mul_spec : forall x y, [|w2_mul x y|] = ([|x|] * [|y|]) mod w2_B.
+Proof.
+ assert (H1: 0 < w2_B). exact (refl_equal Lt).
+ assert (H2: w2_B > 0). exact (refl_equal Gt).
+ unfold w2_mul;intros x y.
+ assert (H := w2_mul_c_spec x y); destruct (w2_mul_c x y).
+ rewrite <- H; reflexivity.
+ rewrite <- H; simpl.
+ rewrite Zmod_plus;trivial.
+ rewrite Zmod_mult;trivial.
+ rewrite Z_mod_same;trivial.
+ rewrite Zmult_0_r; rewrite (Zmod_def_small 0).
+ simpl; rewrite Zmod_mod;trivial.
+ rewrite Zmod_def_small;trivial.
+ apply w2_to_Z_spec.
+ split;[intro Heq;discriminate Heq | exact (refl_equal Lt)].
+Qed.
+
