num/W/W2/W2_op.v
@@ -1,0 +1,28 @@
+Require Export W2_basic.
+Require Export W2_compare.
+Require Export W2_opp.
+Require Export W2_add.
+Require Export W2_sub.
+Require Export W2_mul.
+Require Export W2_div.
+Require Export W2_lift.
+Require Import ZnZ.
+
+
+
+(* ** Record of basic operators for base 4 ** *)
+
+Definition w2_op  :=
+ mk_znz_op 2
+       w2_to_Z w2_of_pos w2_head0
+       OO OI II
+       w2_WW w2_CW
+       w2_compare
+       w2_opp_c w2_opp_carry
+       w2_succ_c
+       w2_add_c w2_add_carry_c w2_add
+       w2_pred_c
+       w2_sub_c w2_sub_carry_c w2_sub
+       w2_mul_c w2_mul w2_square_c
+       w2_div21 w2_add_mul_div.
+
