num/W/W2/W2_op_spec.v
@@ -1,0 +1,54 @@
+Require Import ZArith.
+Open Local Scope Z_scope.
+Require Import W2_basic.
+Require Import W2_basic_spec.
+Open Local Scope w2_scope.
+Require Import W2_op.
+
+
+Require Import W2_opp_spec.
+Require Import W2_compare_spec.
+Require Import W2_succ_c_spec.
+Require Import W2_add_c_spec.
+Require Import W2_add_carry_c_spec.
+Require Import W2_add_spec.
+Require Import W2_pred_c_spec.
+Require Import W2_sub_c_spec.
+Require Import W2_sub_carry_c_spec.
+Require Import W2_sub_spec.
+Require Import W2_mul_c_spec.
+Require Import W2_mul_spec.
+Require Import W2_square_c_spec.
+Require Import W2_div_spec.
+Require Import W2_head0_spec.
+Require Import W2_add_mul_div_spec.
+Require Import ZnZ.
+Lemma w2_op_spec : znz_spec w2_op.
+Proof.
+ apply mk_znz_spec.
+ exact w2_to_Z_spec.
+ exact w2_of_pos_spec.
+ exact w2_0_spec.
+ exact w2_1_spec.
+ exact w2_Bm1_spec.
+ exact w2_WW_spec.
+ exact w2_CW_spec.
+ exact w2_compare_spec.
+ exact w2_opp_c_spec.
+ exact w2_opp_carry_spec.
+ exact w2_succ_c_spec.
+ exact w2_add_c_spec.
+ exact w2_add_carry_c_spec.
+ exact w2_add_spec.
+ exact w2_pred_c_spec.
+ exact w2_sub_c_spec.
+ exact w2_sub_carry_c_spec.
+ exact w2_sub_spec.
+ exact w2_mul_c_spec.
+ exact w2_mul_spec.
+ exact w2_square_c_spec.
+ exact w2_div21_spec.
+ exact w2_head0_spec.
+ exact w2_add_mul_div_spec.
+Qed.
+
