num/W/W2/W2_pred_c_spec.v
@@ -1,0 +1,17 @@
+Require Import ZArith.
+Open Local Scope Z_scope.
+Require Import W2_basic.
+Open Local Scope w2_scope.
+Require Import W2_sub.
+
+
+Lemma w2_pred_c_spec : forall x,  [-|w2_pred_c x|] = [|x|] - 1.
+Proof
+fun x =>
+ match x as x return  [-|w2_pred_c x|] = [|x|] - 1 with
+ | OO => refl_equal (-1)
+ | OI => refl_equal (0)
+ | IO => refl_equal (1)
+ | II => refl_equal (2)
+ end.
+
