num/W/W2/W2_sub_c_spec.v
@@ -1,0 +1,41 @@
+Require Import ZArith.
+Open Local Scope Z_scope.
+Require Import W2_basic.
+Open Local Scope w2_scope.
+Require Import W2_sub.
+
+
+Lemma w2_sub_c_spec : forall x y, [-|w2_sub_c x y|] = [|x|] - [|y|].
+Proof
+fun x y =>
+ match y as y return [-|w2_sub_c x y|] = [|x|] - [|y|] with
+ | OO =>
+    match x as x return [-|w2_sub_c x OO|] = [|x|] - [|OO|] with
+    | OO => refl_equal (0)
+    | OI => refl_equal (1)
+    | IO => refl_equal (2)
+    | II => refl_equal (3)
+   end
+ | OI =>
+    match x as x return [-|w2_sub_c x OI|] = [|x|] - [|OI|] with
+    | OO => refl_equal (-1)
+    | OI => refl_equal (0)
+    | IO => refl_equal (1)
+    | II => refl_equal (2)
+   end
+ | IO =>
+    match x as x return [-|w2_sub_c x IO|] = [|x|] - [|IO|] with
+    | OO => refl_equal (-2)
+    | OI => refl_equal (-1)
+    | IO => refl_equal (0)
+    | II => refl_equal (1)
+   end
+ | II =>
+    match x as x return [-|w2_sub_c x II|] = [|x|] - [|II|] with
+    | OO => refl_equal (-3)
+    | OI => refl_equal (-2)
+    | IO => refl_equal (-1)
+    | II => refl_equal (0)
+   end
+ end.
+
